theories/IL/VarP.v
@@ -1,0 +1,33 @@
+Require Import Var IL.
+
+Inductive var_P (P:var -> Prop)
+  : stmt -> Prop :=
+| VarPOpr x b e
+  :  var_P P b
+     -> P x
+     -> For_all P (Exp.freeVars e)
+     -> var_P P (stmtLet x e b)
+| VarPIf e b1 b2
+  :  For_all P (Op.freeVars e)
+     -> var_P P b1
+     -> var_P P b2
+     -> var_P P (stmtIf e b1 b2)
+| VarPGoto l Y
+  : For_all P (list_union (Op.freeVars ⊝ Y))
+    -> var_P P (stmtApp l Y)
+| VarPReturn e
+  : For_all P (Op.freeVars e)
+    -> var_P P (stmtReturn e)
+| VarPLet F b
+  : (forall n Zs, get F n Zs -> var_P P (snd Zs))
+    -> (forall n Zs, get F n Zs -> For_all P (of_list (fst Zs)))
+    -> var_P P b
+    -> var_P P (stmtFun F b).
+
+Lemma var_P_occurVars (P:var -> Prop) s
+  : var_P P s
+    -> For_all P (occurVars s).
+Proof.
+  induction 1; unfold For_all in *; intros; simpl in *; cset_tac'.
+  eapply list_union_get in H4. destruct H4; dcr; inv_get; cset_tac.
+Qed.
