theories/Spilling/Spilling.v
@@ -1,6 +1,7 @@
 Require Import Util CSet MapDefined AllInRel.
-Require Import Var MapInjectivity IL Annotation AnnP Sim.
+Require Import Var MapInjectivity IL Annotation AnnP Sim LabelsDefined.
 Require Import SimplSpill SpillSound SpillSim DoSpill DoSpillRm Take Drop.
+Require Import Coherence.
 Require Import ExpVarsBounded ReconstrLive ReconstrLiveSmall ReconstrLiveSound.
 Require Import Liveness RenamedApart RenameApart_Liveness AddParams Slot.
 
@@ -41,20 +42,6 @@ Definition spill (k:nat) (slot:var -> var)
   let s_fun := addParams s_spilled lv_spilled in
   (s_fun, lv_spilled).
 
-Lemma of_list_drop_incl X `{OrderedType X} (n : nat) (L:list X)
-  : of_list (drop n L) ⊆ of_list L.
-Proof.
-  general induction L; destruct n; simpl; eauto with cset.
-  rewrite drop_nil; eauto.
-Qed.
-
-Lemma of_list_drop_elements_incl X `{OrderedType X} (n : nat) (s : set X)
-  : of_list (drop n (elements s)) ⊆ s.
-Proof.
-  rewrite of_list_drop_incl.
-  rewrite of_list_elements; eauto.
-Qed.
-
 Lemma agree_on_update_list_slot X `{OrderedType X} Y (L:list X) (L':list Y) (V:X->Y)
       `{Proper _ (_eq ==> eq) V} f `{Proper _ (_eq ==> _eq) f} V' D (Len:❬L❭= ❬L'❭)
   :  agree_on eq (D \ of_list L) V (fun x => V' (f x))
@@ -76,15 +63,15 @@ Proof.
     cset_tac'. eapply H4 in H8; eauto; cset_tac.
 Qed.
 
-Lemma spill_correct b k (kGT:k > 0) (s:stmt) lv ra E
-      (PM:LabelsDefined.paramsMatch s nil)
+Lemma spill_correct b k (s:stmt) lv ra E
+      (PM:paramsMatch s nil)
       (LV:Liveness.live_sound Liveness.Imperative nil nil s lv)
       (AEF:AppExpFree.app_expfree s)
       (RA:RenamedApart.renamedApart s ra)
       (Def:defined_on (getAnn lv) E)
       (Bnd:exp_vars_bounded k s)
       (Incl:getAnn lv ⊆ fst (getAnn ra))
-      (NUC:LabelsDefined.noUnreachableCode (LabelsDefined.isCalled b) s)
+      (NUC:noUnreachableCode (isCalled b) s)
       (slt:Slot (fst (getAnn ra) ∪ snd (getAnn ra)))
       (aIncl:ann_R (fun (x : ⦃var⦄) (y : ⦃var⦄ * ⦃var⦄) => x ⊆ fst y) lv ra)
   : sim I.state F.state bot3 Sim
@@ -180,14 +167,14 @@ Proof.
     + eapply (@do_spill_no_unreachable_code _ _ _ _ nil nil); eauto.
 Qed.
 
-Lemma spill_live b k (kGT:k > 0) (s:stmt) lv ra
-      (PM:LabelsDefined.paramsMatch s nil)
+Lemma spill_live b k (s:stmt) lv ra
+      (PM:paramsMatch s nil)
       (LV:Liveness.live_sound Liveness.Imperative nil nil s lv)
       (AEF:AppExpFree.app_expfree s)
       (RA:RenamedApart.renamedApart s ra)
       (Bnd:exp_vars_bounded k s)
       (Incl:getAnn lv ⊆ fst (getAnn ra))
-      (NUC:LabelsDefined.noUnreachableCode (LabelsDefined.isCalled b) s)
+      (NUC:noUnreachableCode (isCalled b) s)
       (slt:Slot (fst (getAnn ra) ∪ snd (getAnn ra)))
       (aIncl:ann_R (fun (x : ⦃var⦄) (y : ⦃var⦄ * ⦃var⦄) => x ⊆ fst y) lv ra)
   : live_sound FunctionalAndImperative
@@ -234,4 +221,170 @@ Proof.
     ** reflexivity.
     ** isabsurd.
   - eapply (@do_spill_no_unreachable_code _ _ _ _ nil nil); eauto.
+Qed.
+
+Require Import MoreTac.
+
+Lemma spill_srd b k (s:stmt) lv ra
+      (PM:paramsMatch s nil)
+      (LV:Liveness.live_sound Liveness.Imperative nil nil s lv)
+      (AEF:AppExpFree.app_expfree s)
+      (RA:RenamedApart.renamedApart s ra)
+      (Bnd:exp_vars_bounded k s)
+      (Incl:getAnn lv ⊆ fst (getAnn ra))
+      (NUC:noUnreachableCode (isCalled b) s)
+      (slt:Slot (fst (getAnn ra) ∪ snd (getAnn ra)))
+      (aIncl:ann_R (fun (x : ⦃var⦄) (y : ⦃var⦄ * ⦃var⦄) => x ⊆ fst y) lv ra)
+  : srd nil (fst (spill k slt s lv)) (snd (spill k slt s lv)).
+Proof.
+  unfold spill.
+  set (R:=of_list (take k (to_list (getAnn lv)))).
+  set (M:=of_list (drop k (to_list (getAnn lv)))).
+  set (spl:=(simplSpill k nil nil R M s lv)).
+  set (VD:=fst (getAnn ra) ∪ snd (getAnn ra)).
+  assert (lvRM:getAnn lv [=] R ∪ M). {
+    subst R M. rewrite <- of_list_app. rewrite <- take_eta.
+    rewrite of_list_3. eauto.
+  }
+  assert (SPS:spill_sound k nil nil (R, M) s spl). {
+    eapply simplSpill_sat_spillSound; eauto using PIR2.
+    subst R. rewrite TakeSet.take_of_list_cardinal; eauto.
+    rewrite lvRM; eauto.
+  }
+  assert (Disj: disj R M). {
+    subst R M. clear. hnf; intros.
+    eapply of_list_get_first in H; dcr. cset_tac'.
+    eapply of_list_get_first in H0; dcr; cset_tac'.
+    inv_get.
+    refine (NoDupA_get_neq' _ _ H0 H _); eauto.
+    eapply (elements_3w (getAnn lv)).
+    omega.
+  }
+  assert (InclR: R ⊆ VD). {
+    subst R VD. unfold to_list.
+    rewrite TakeSet.take_set_incl. eauto with cset.
+  }
+  assert (InclM: M ⊆ VD). {
+    subst M VD. unfold to_list.
+    rewrite of_list_drop_elements_incl. eauto with cset.
+  }
+  assert (spl_lv:SpillSound.spill_live VD spl lv). {
+    eapply simplSpill_spill_live; eauto using lv_ra_lv_bnd.
+  }
+  eapply addParams_srd; eauto.
+  - eapply (@reconstr_live_sound k _ slt nil _ nil R M); eauto using PIR2.
+    ** reflexivity.
+    ** isabsurd.
+  - eapply (@do_spill_no_unreachable_code _ _ _ _ nil nil); eauto.
+Qed.
+
+Lemma spill_paramsMatch b k (s:stmt) lv ra
+      (PM:paramsMatch s nil)
+      (LV:Liveness.live_sound Liveness.Imperative nil nil s lv)
+      (AEF:AppExpFree.app_expfree s)
+      (RA:RenamedApart.renamedApart s ra)
+      (Bnd:exp_vars_bounded k s)
+      (Incl:getAnn lv ⊆ fst (getAnn ra))
+      (NUC:noUnreachableCode (isCalled b) s)
+      (slt:Slot (fst (getAnn ra) ∪ snd (getAnn ra)))
+      (aIncl:ann_R (fun (x : ⦃var⦄) (y : ⦃var⦄ * ⦃var⦄) => x ⊆ fst y) lv ra)
+  : paramsMatch (fst (spill k slt s lv)) nil.
+Proof.
+  unfold spill; simpl.
+  set (R:=of_list (take k (to_list (getAnn lv)))).
+  set (M:=of_list (drop k (to_list (getAnn lv)))).
+  set (spl:=(simplSpill k nil nil R M s lv)).
+  set (VD:=fst (getAnn ra) ∪ snd (getAnn ra)).
+  assert (lvRM:getAnn lv [=] R ∪ M). {
+    subst R M. rewrite <- of_list_app. rewrite <- take_eta.
+    rewrite of_list_3. eauto.
+  }
+  assert (SPS:spill_sound k nil nil (R, M) s spl). {
+    eapply simplSpill_sat_spillSound; eauto using PIR2.
+    subst R. rewrite TakeSet.take_of_list_cardinal; eauto.
+    rewrite lvRM; eauto.
+  }
+  assert (Disj: disj R M). {
+    subst R M. clear. hnf; intros.
+    eapply of_list_get_first in H; dcr. cset_tac'.
+    eapply of_list_get_first in H0; dcr; cset_tac'.
+    inv_get.
+    refine (NoDupA_get_neq' _ _ H0 H _); eauto.
+    eapply (elements_3w (getAnn lv)).
+    omega.
+  }
+  assert (InclR: R ⊆ VD). {
+    subst R VD. unfold to_list.
+    rewrite TakeSet.take_set_incl. eauto with cset.
+  }
+  assert (InclM: M ⊆ VD). {
+    subst M VD. unfold to_list.
+    rewrite of_list_drop_elements_incl. eauto with cset.
+  }
+  assert (spl_lv:SpillSound.spill_live VD spl lv). {
+    eapply simplSpill_spill_live; eauto using lv_ra_lv_bnd.
+  }
+  eapply addParams_paramsMatch; eauto.
+  - eapply (@do_spill_paramsMatch _ _ _ nil nil); eauto.
+    isabsurd.
+  - eapply (@reconstr_live_sound k _ slt nil _ nil R M); eauto using PIR2.
+    ** reflexivity.
+    ** isabsurd.
+  - eapply (do_spill_no_unreachable_code _ slt k (R,M) nil nil); eauto.
+Qed.
+
+
+Lemma spill_noUnreachableCode b k (s:stmt) lv ra
+      (PM:paramsMatch s nil)
+      (LV:Liveness.live_sound Liveness.Imperative nil nil s lv)
+      (AEF:AppExpFree.app_expfree s)
+      (RA:RenamedApart.renamedApart s ra)
+      (Bnd:exp_vars_bounded k s)
+      (Incl:getAnn lv ⊆ fst (getAnn ra))
+      (NUC:noUnreachableCode (isCalled b) s)
+      (slt:Slot (fst (getAnn ra) ∪ snd (getAnn ra)))
+      (aIncl:ann_R (fun (x : ⦃var⦄) (y : ⦃var⦄ * ⦃var⦄) => x ⊆ fst y) lv ra)
+  : noUnreachableCode (isCalled b) (fst (spill k slt s lv)).
+Proof.
+  unfold spill; simpl.
+  set (R:=of_list (take k (to_list (getAnn lv)))).
+  set (M:=of_list (drop k (to_list (getAnn lv)))).
+  set (spl:=(simplSpill k nil nil R M s lv)).
+  set (VD:=fst (getAnn ra) ∪ snd (getAnn ra)).
+  assert (lvRM:getAnn lv [=] R ∪ M). {
+    subst R M. rewrite <- of_list_app. rewrite <- take_eta.
+    rewrite of_list_3. eauto.
+  }
+  assert (SPS:spill_sound k nil nil (R, M) s spl). {
+    eapply simplSpill_sat_spillSound; eauto using PIR2.
+    subst R. rewrite TakeSet.take_of_list_cardinal; eauto.
+    rewrite lvRM; eauto.
+  }
+  assert (Disj: disj R M). {
+    subst R M. clear. hnf; intros.
+    eapply of_list_get_first in H; dcr. cset_tac'.
+    eapply of_list_get_first in H0; dcr; cset_tac'.
+    inv_get.
+    refine (NoDupA_get_neq' _ _ H0 H _); eauto.
+    eapply (elements_3w (getAnn lv)).
+    omega.
+  }
+  assert (InclR: R ⊆ VD). {
+    subst R VD. unfold to_list.
+    rewrite TakeSet.take_set_incl. eauto with cset.
+  }
+  assert (InclM: M ⊆ VD). {
+    subst M VD. unfold to_list.
+    rewrite of_list_drop_elements_incl. eauto with cset.
+  }
+  assert (spl_lv:SpillSound.spill_live VD spl lv). {
+    eapply simplSpill_spill_live; eauto using lv_ra_lv_bnd.
+  }
+  eapply addParams_noUnreachableCode; eauto.
+  - eapply (@do_spill_paramsMatch _ _ _ nil nil); eauto.
+    isabsurd.
+  - eapply (@reconstr_live_sound k _ slt nil _ nil R M); eauto using PIR2.
+    ** reflexivity.
+    ** isabsurd.
+  - eapply (do_spill_no_unreachable_code _ slt k (R,M) nil nil); eauto.
 Qed.
